SEQ adeqaucy - WIP deflat

src/prop/Pred.v
@@ -30,6 +30,31 @@ Section Pred.
 
   Definition te_pred := ThreadEvent.t -> Prop.
 
+  Definition is_promise (e: ThreadEvent.t): Prop :=
+    match e with
+    | ThreadEvent.promise _ _ _ _ _ => True
+    | _ => False
+    end.
+
+  Definition release_event (e: ThreadEvent.t): Prop :=
+    match e with
+    | ThreadEvent.update _ _ _ _ _ _ _ _ ordw => Ordering.le Ordering.strong_relaxed ordw
+    | ThreadEvent.write _ _ _ _ _ ord => Ordering.le Ordering.strong_relaxed ord
+    | ThreadEvent.fence _ ordw => Ordering.le Ordering.strong_relaxed ordw
+    | ThreadEvent.syscall _ => True
+    | ThreadEvent.failure => True
+    | ThreadEvent.racy_write _ _ _ => True
+    | ThreadEvent.racy_update _ _ _ _ _ => True
+    | _ => False
+    end.
+
+  Definition is_na_write (e: ThreadEvent.t): Prop :=
+    match e with
+    | ThreadEvent.na_write _ _ _ _ _ _ _ => True
+    | ThreadEvent.write _ _ _ _ _ ord => Ordering.le ord Ordering.na
+    | _ => False
+    end.
+
   Definition promise_free (e: ThreadEvent.t): Prop :=
     match e with
     | ThreadEvent.promise loc from to msg kind =>
