src/gsim/DelayedSimulation.v
@@ -33,6 +33,7 @@ Require Import Program.
 Require Import JoinedView.
 Require Import gSimAux.
 Require Import gSimulation.
+Require Import Pred.
 Require Import Delayed.
 Require Import LowerMemory.
 
